frodo/code/Hacl.Frodo.KEM.fst
@@ -14,6 +14,8 @@ open Hacl.Impl.Matrix
 open Hacl.Impl.Frodo.Params
 open Hacl.Impl.Frodo.KEM
 
+module S = Frodo.KEM
+
 #reset-options "--z3rlimit 50 --max_fuel 0 --max_ifuel 0 --using_facts_from '* -FStar.Seq'"
 
 val crypto_kem_keypair:
@@ -21,8 +23,10 @@ val crypto_kem_keypair:
   -> sk:lbytes crypto_secretkeybytes
   -> Stack uint32
     (requires fun h -> live h pk /\ live h sk /\ disjoint pk sk)
-    (ensures  fun h0 r h1 -> live h1 pk /\ live h1 sk /\
-      modifies (loc_union (loc_buffer pk) (loc_buffer sk)) h0 h1)
+    (ensures  fun h0 r h1 ->
+      modifies (loc_union (loc_buffer pk) (loc_buffer sk)) h0 h1 /\
+      (let pk_s, sk_s = S.crypto_kem_keypair () in
+      as_seq h1 pk == pk_s /\ as_seq h1 sk == sk_s))
 let crypto_kem_keypair pk sk = Hacl.Impl.Frodo.KEM.KeyGen.crypto_kem_keypair pk sk
 
 val crypto_kem_enc:
@@ -33,7 +37,10 @@ val crypto_kem_enc:
     (requires fun h ->
       live h ct /\ live h ss /\ live h pk /\
       disjoint ct ss /\ disjoint ct pk /\ disjoint ss pk)
-    (ensures  fun h0 _ h1 -> modifies (loc_union (loc_buffer ct) (loc_buffer ss)) h0 h1)
+    (ensures  fun h0 _ h1 ->
+      modifies (loc_union (loc_buffer ct) (loc_buffer ss)) h0 h1 /\
+      (let ct_s, ss_s = S.crypto_kem_enc (as_seq h0 pk) in
+      as_seq h1 ct == ct_s /\ as_seq h1 ss == ss_s))
 let crypto_kem_enc ct ss pk = Hacl.Impl.Frodo.KEM.Encaps.crypto_kem_enc ct ss pk
 
 val crypto_kem_dec:
@@ -44,5 +51,7 @@ val crypto_kem_dec:
     (requires fun h ->
       live h ss /\ live h ct /\ live h sk /\
       disjoint ss ct /\ disjoint ss sk /\ disjoint ct sk)
-    (ensures  fun h0 r h1 -> live h1 ss /\ modifies (loc_buffer ss) h0 h1)
+    (ensures  fun h0 r h1 ->
+      modifies (loc_buffer ss) h0 h1 /\
+      as_seq h1 ss == S.crypto_kem_dec (as_seq h0 ct) (as_seq h0 sk))
 let crypto_kem_dec ss ct sk = Hacl.Impl.Frodo.KEM.Decaps.crypto_kem_dec ss ct sk
