frodo/spec/Frodo.KEM.fst
@@ -1,0 +1,24 @@
+module Frodo.KEM
+
+open Lib.IntTypes
+open Lib.Sequence
+open Lib.ByteSequence
+
+open Spec.Frodo.Params
+open Spec.Frodo.KEM
+
+val crypto_kem_keypair:
+     unit
+  -> tuple2 (lbytes crypto_publickeybytes) (lbytes crypto_secretkeybytes)
+let crypto_kem_keypair () = Spec.Frodo.KEM.KeyGen.crypto_kem_keypair ()
+
+val crypto_kem_enc:
+    pk:lbytes crypto_publickeybytes
+  -> tuple2 (lbytes crypto_ciphertextbytes) (lbytes crypto_bytes)
+let crypto_kem_enc pk = Spec.Frodo.KEM.Encaps.crypto_kem_enc pk
+
+val crypto_kem_dec:
+     ct:lbytes crypto_ciphertextbytes
+  -> sk:lbytes crypto_secretkeybytes
+  -> ss:lbytes crypto_bytes
+let crypto_kem_dec ct sk = Spec.Frodo.KEM.Decaps.crypto_kem_dec ct sk
