frodo/spec/Spec.Frodo.Random.fst
@@ -1,0 +1,9 @@
+module Spec.Frodo.Random
+
+open Lib.IntTypes
+open Lib.Sequence
+
+//val randombytes_init_: entropy_input:lseq uint8 48 -> unit
+
+val randombytes_: len:size_nat -> res:lseq uint8 len
+let randombytes_ len = create len (u8 0) //Just to extract the spec
